---
title: Response and Correlation
number-sections: false
format:
  revealjs:
    theme: [default, reveal_custom.scss]
    slide-number: true
    hash: true
    center: true
    auto-stretch: false
    html-math-method: katex
    preview-links: true
    katex: {
      throwOnError: false,
    }
---

{{< include ../macros.qmd >}}

# Response & Correlation

- Calculating eigenstates and eigenenergies is one thing, but what do experimentalists actually measure?

- Want to understand how many body systems _respond_ dynamically to an external probe

- Time evolution of _spontaneous fluctuations_ (thermal or quantum) obeys similar dynamics $\longrightarrow$ __fluctuationâ€“dissipation relation__


---

### Quantum fluctuations: one oscillator

- For a single (undamped) oscillator we have ground state fluctuations
$$
H = \frac{p^2}{2m} + \frac{1}{2}m\omega_0^2 y^2
$$
$$
\bra{0} y^2 \ket{0} = \frac{1}{2m \omega_0}
$$

---

- At finite temperature
$$
\langle\langle y^2\rangle\rangle=\tr\left[\rho\\, y^2\right] = \frac{\coth(\beta\omega_0/2)}{2m\omega_0}
$$
$\rho = e^{-\beta H}/Z$ is equilibrium density matrix, and $Z=\tr[e^{-\beta H}]$ is partition function

- The double angular brackets $\langle\langle (\cdots)\rangle\rangle$ denote that we are taking quantum _and thermal_ expectations.

---

- What about _time dependent fluctuations_? A natural candidate:
$$
\langle\langle y(t)y(0)\rangle\rangle,
$$
$y(t) = e^{iHt} y e^{-iHt}$ (Heisenberg picture) 

- This gives the _quantum_ noise spectrum

$$
S(\omega) = \int_{-\infty}^\infty \langle\langle y(t)y(0)\rangle\rangle e^{i\omega t}\,dt.
$$

- __BUT__: since $y(0)$ and $y(t)$ do not commute with each other $\langle\langle y(t)y(0)\rangle\rangle\neq \langle\langle y(0)y(t)\rangle\rangle=\langle\langle y(-t)y(0)\rangle\rangle$, so

$$
S(\omega)\neq S(-\omega)
$$

---

- Many of the properties of $S(\omega)$ are most easily understood from __spectral representation__

-  Insert complete set of energy eigenstates between $y(0)$ and $y(t)$

$$
S(\omega) = 2\pi\sum_{m,n} \frac{e^{-\beta E_n}}{Z} |\bra{n}y\ket{m}|^2 \delta(\omega-E_m+E_n)
$$

- Reason for asymmetry in $S(\omega)$ is that term with $\delta(\omega-E_m+E_n)$ is weighted by $e^{-\beta E_n}$, while term with $\delta(\omega-E_n+E_m)$ has $e^{-\beta E_m}$


$$
S(\omega) = S(-\omega) e^{\beta\omega}.
$$


---

- At zero temperature $\beta\to\infty$ and we can see that $S(\omega<0)=0$.

- Let's evaluate $S(\omega)$ for oscillator. The matrix elements are
$$
\bra{n}y\ket{m} = \frac{1}{\sqrt{2m\omega_0}}\begin{cases}
\sqrt{m+1} & \text{if } n=m+1 \\
\sqrt{m} & \text{if } n=m-1.
\end{cases}
$$
$$
\begin{align*}
S(\omega)&=\frac{\pi}{m\omega_0} \sum_n \frac{e^{-\beta E_n}}{Z} \left[n\delta(\omega+\omega_0)+(n+1)\delta(\omega-\omega_0)\right]\nonumber\\
& = \frac{\pi}{m\omega_0}\left[n_\text{B}(\omega_0)\delta(\omega+\omega_0)+(n_\text{B}(\omega_0)+1)\delta(\omega-\omega_0)\right]
\end{align*}
$$
$$
n_\text{B}(\omega)\equiv \frac{1}{\exp\left(\beta\omega\right)-1}
$$
is Bose distribution function

---

$$
\begin{align*}
S(\omega)&=\frac{\pi}{m\omega_0} \sum_n \frac{e^{-\beta E_n}}{Z} \left[n\delta(\omega+\omega_0)+(n+1)\delta(\omega-\omega_0)\right]\nonumber\\
& = \frac{\pi}{m\omega_0}\left[n_\text{B}(\omega_0)\delta(\omega+\omega_0)+(n_\text{B}(\omega_0)+1)\delta(\omega-\omega_0)\right]
\end{align*}
$$

- Shows the predicted asymmetry between positive and negative frequencies. We can check that
$$
\int S(\omega)\frac{d\omega}{2\pi} = \langle\langle y^2\rangle\rangle= \frac{\coth(\beta\omega_0/2)}{2m\omega_0}
$$
as we found before.

---

### Classical limit $\beta\omega\to 0$

$$
\begin{align*}
S(\omega)&= \frac{\pi}{m\omega_0}\left[n_\text{B}(\omega_0)\delta(\omega+\omega_0)+(n_\text{B}(\omega_0)+1)\delta(\omega-\omega_0)\right]\\\\
&\to \frac{k_\text{B}T}{2m\omega_0^2} \times 2\pi\left[\delta(\omega+\omega_0)+\delta(\omega-\omega_0)\right]
\end{align*}
$$

- Consistent with equipartition: $\frac{1}{2}m\omega_0^2 \langle y^2\rangle=\frac{1}{2}k_\text{B}T$

---

### Many oscillators

- We can express  $y(t)$ in terms of normal modes as
$$
y(t) = \sum_k \left[c^{}_k \adop_k(t) + c_k^* \aop_k(t)\right]
$$
- Time evolution of mode operators is

$$
\adop_k(t) = e^{i\omega_k t}\adop_k,\quad \aop_k(t) = e^{-i\omega_k t}\aop_k
$$

- Repeating calculation of $S(\omega)$ gives

$$
\begin{align*}
S(\omega)= 2\pi\sum_k |c_k|^2\left[n_\text{B}(\omega_k)\delta(\omega+\omega_k)+(n_\text{B}(\omega_k)+1)\delta(\omega-\omega_k)\right]
\end{align*}
$$

- In continuum limit sum of $\delta(\omega\pm\omega_k)\longrightarrow$ smooth $S(\omega)$

---

### Response of oscillator system

- Solve Heisenberg equations of motion 
$$
H = \sum_k \omega_k \adop_k\aop_k - f(t)y,
$$
where $y$ is written in terms of normal modes
$$
\frac{d\aop_k}{dt} = -i\omega_k \aop_k +i c_k f(t),
$$

- Solution is $\aop_k(t) = e^{-i\omega_k t}\aop_k(0)+a_{k,f}(t)$ with
$$
\aop_{k,f}(\omega) \equiv \frac{c_k}{\omega_k-\omega-i0} f(\omega).
$$
($-i0$ introduced for response analytic in UHP i.e. causal)

---

- Response of $\aop_k(t)\longrightarrow y(t)$ gives

$$
y(\omega) = \sum_k |c_k|^2\left[\frac{1}{\omega_k-\omega-i0}+\frac{1}{\omega_k+\omega+i0}\right]f(\omega).
$$

- This defines the __response function__ $\chi(\omega)$
$$
\chi(\omega)\equiv \frac{y(\omega)}{f(\omega)} = \sum_k |c_k|^2\left[\frac{1}{\omega_k-\omega-i0}+\frac{1}{\omega_k+\omega+i0}\right]
$$

- Then use... 

$$
\text{Im} \frac{1}{x\mp i0} = \pm\pi\delta(x),
$$

---

$$
\operatorname{Im}\chi(\omega) =\sgn(\omega)\pi\sum_k |c_k|^2\delta(\omega_k-\omega) 
$$

- $S(\omega)$ and $\operatorname{Im}\chi(\omega)$ are then related by

$$
S(\omega) = 2\operatorname{Im}\chi(\omega)\left[n_\text{B}(\omega)+1\right]
$$

- This is a __quantum fluctuation dissipation relation__

---

::: {.callout-tip}
## Check

Check that in the classical limit ($k_\text{B}T\gg \hbar \omega$)
$$
S(\omega) = 2\operatorname{Im}\chi(\omega)\left[n_\text{B}(\omega)+1\right]
$$
reduces to 
$$
S(\omega)=\frac{2k_\text{B}T}{\omega} \operatorname{Im}\chi(\omega)
$$
Consistent with classical equipartition

:::

---

### Golden Rule and Dissipation

- We saw that classically $\text{Im}\,\chi(\omega)$ related to dissipation

- FDT relates $\operatorname{Im}\chi(\omega)$ and $S(\omega)$. How is $S(\omega)$ related to dissipation?

- Regard driving force as perturbation that causes transitions between energy eigenstates
$$
H_\text{pert} = - f(t)y
$$
with $f(t)=f_0\cos\omega t$

---

- In lowest order perturbation theory, system makes transitions $\pm\omega$ in energy

- Rates found from Fermi's golden rule

$$
\Gamma_{n\to m} = 2\pi \left(\frac{f_0}{2}\right)^2|\bra{n}y\ket{m}|^2 \delta(\pm\omega+E_m-E_n).
$$


- Total rate is sum over all initial ($\ket{n}$) and final states ($\ket{m}$), including probability $e^{-\beta E_n}/Z$ of finding the system initially in $\ket{n}$

- c.f. spectral representation of $S(\omega)$

$$
S(\omega) = 2\pi\sum_{m,n} \frac{e^{-\beta E_n}}{Z} |\bra{n}y\ket{m}|^2 \delta(\omega-E_m+E_n)
$$

$$
\Gamma(\omega) = S(\omega)\left(\frac{f_0}{2}\right)^2
$$

---

- $S(\omega)$ measures rate of transitions _absorbing_ energy $\omega$; $S(-\omega)$ the rate for _emitting_ energy $\omega$. 

- Asymmetry of $S(\omega)$ is asymmetry between emission and absorption of radiation

- The rate of energy absorption is

$$
\omega\Gamma(\omega) = \omega S(\omega)\left(\frac{f_0}{2}\right)^2 = \frac{1}{2}\omega\operatorname{Im}\chi(\omega)\left[n_\text{B}(\omega)+1\right]f_0^2
$$

---

$$
\omega\Gamma(\omega) = \omega S(\omega)\left(\frac{f_0}{2}\right)^2 = \frac{1}{2}\omega\operatorname{Im}\chi(\omega)\left[n_\text{B}(\omega)+1\right]f_0^2
$$

::: {.callout-tip}
## Check

Compare with 
$$
\begin{align*}
W_\text{diss} = \langle f(t) \dot y(t)\rangle = \frac{1}{2}\omega\operatorname{Im}\chi(\omega)f_0^2
\end{align*}
$$
They agree when $n_\text{B}(\omega)\to 0$: energy of transition being much larger than thermal energy $\hbar\omega\gg k_B T$.

:::

---

## Linear Response: Formal Theory

- So far, considered only response of _linear systems_!

- How do we talk about linear response _in general_?

---

### Kubo Formula

- How does observable $A$ depend on $\lambda_t$, which appears (for small variations) linearly in the Hamiltonian

$$
H_t = H_0 - \lambda_t B?
$$

- $B=-\frac{\partial H}{\partial \lambda}$ is __generalized force__; $\lambda$ __generalized displacement__

---

- In the interaction picture $\ket{\Psi_I(t)} \equiv e^{iH_0 t}\ket{\Psi(t)}$
$$
i\frac{\partial \ket{\Psi_I(t)}}{\partial t} = -\lambda_t B_I(t) \ket{\Psi_I(t)},
$$
where $B_I(t) = e^{iH_0 t}B e^{-iH_0 t}$

- Result of first order time dependent perturbation theory is $\ket{\Psi_I(t)}=\ket{\Psi(0)}+\ket{\Psi^{(1)}_I(t)}+\cdots$, with

$$
\ket{\Psi^{(1)}_I(t)} = i\int_0^t dt' \lambda_{t'} B_I(t') \ket{\Psi(0)}
$$

$$
\begin{align*}
&\Braket{\Psi(t)|A|\Psi(t)} = \Braket{\Psi_I(t)|A_I(t) |\Psi_I(t)} \nonumber\\
&=\Braket{\Psi(0)|A_I(t)|\Psi(0)} +i \int_0^t dt' \lambda_{t'}\Braket{\Psi(0)| \left[A_I(t),B_I(t')\right] |\Psi(0)}
\end{align*}
$$

---

- Mixed states can be treated by averaging over a distribution of quantum states $\langle\cdots \rangle \longrightarrow \langle\langle\cdots\rangle\rangle$

- $\chi_{AB}(t)$ of $A$ due to perturbation that couples to $B$

$$
\chi_{AB}(t) = i\langle\langle\left[A_I(t),B_I(0)\right]\rangle\rangle,\quad t>0.
$$
(Normally write $A(t)$ rather than $A_I(t)$: Heisenberg picture for the unperturbed problem) 

- This is the __Kubo formula__. It expresses the response of a system in terms of the dynamics of the unperturbed system.

---

### Fluctuation Dissipation Theorem (general)
 
- Start from the correlation function

$$
S_{AB}(t) \equiv \langle\langle A_I(t)B_I(0)\rangle\rangle
$$

- Recalling that $\langle\langle\cdots \rangle\rangle = \frac{1}{Z}\tr\left[e^{-\beta H}\cdots\right]$, you should be able to show that

$$
S_{AB}(t) = S_{BA}(-t-i\beta)
$$

::: {.callout-tip}
## Check

Hint: use the cyclic property of the trace.

:::

---

$$
S_{AB}(t) = S_{BA}(-t-i\beta).
$$

- Fourier transforming, we arrive at

$$
S_{AB}(\omega) = e^{\beta\omega} S_{BA}(-\omega)
$$
(we've seen this before!)

- $\chi_{AB}(t)$ (a commutator) can be written in terms of $S_{AB}(\omega)$

$$
\begin{align*}
\chi_{AB}(t) &= \begin{cases}
i\left[S_{AB}(t)-S_{BA}(-t)\right] & t>0\\
0 & t<0
\end{cases}\\
&= i\theta(t)\left[S_{AB}(t)-S_{BA}(-t)\right]
\end{align*}
$$

---

$$
\chi_{AB}(t)=i\theta(t)\left[S_{AB}(t)-S_{BA}(-t)\right]
$$

- $\chi_{AB}(\omega)$ can then be expressed as the convolution. The Fourier transform of the step function is

$$
\tilde\theta(\omega) = \frac{i}{\omega+i0}
$$
$$
\begin{align*}
\chi_{AB}(\omega)&= -\int \frac{d\omega'}{2\pi}\frac{S_{AB}(\omega')-S_{BA}(-\omega')}{\omega-\omega'+i0}\\
&=-\int \frac{d\omega'}{2\pi}\frac{S_{AB}(\omega')\left[1-e^{-\beta\omega'}\right]}{\omega-\omega'+i0}
\end{align*}
$$

---

- To make sense of this formula, use the Kramers--Kronig relation
$$
\begin{align*}
\chi_{AB}(\omega) &=\operatorname{Re}\chi_{AB}(\omega) + i\operatorname{Im}\chi_{AB}(\omega)\\
&= \cP \int_{-\infty}^\infty \frac{d\omega'}{\pi}\frac{\operatorname{Im}\chi_{AB}(\omega')}{\omega'-\omega} + i\operatorname{Im}\chi_{AB}(\omega)\\
&= \int_{-\infty}^\infty \frac{d\omega'}{\pi}\frac{\operatorname{Im}\chi_{AB}(\omega')}{\omega'-\omega-i0},
\end{align*}
$$
where we used
$$
\frac{1}{x+i0} = \cP\frac{1}{x} -i\pi\delta(x)
$$
- Finally!
$$
S_{AB}(\omega) = 2\operatorname{Im}\chi_{AB}(\omega)\left[n_\text{B}(\omega)+1\right]
$$

---

### Spectral Representation

The quantites $\chi_{AB}(\omega)$ and $S_{AB}(\omega)$ have spectral representations in terms of energy eigenstates and eigenvalues

$$
S_{AB}(\omega)  = 2\pi\sum_{m,n} \frac{e^{-\beta E_m}}{Z} \Braket{m|A|n}\Braket{n|B|m} \delta(\omega-E_n+E_m)
$$

::: {.callout-tip}
## Check

Use the spectral representation to prove the fluctuation dissipation relation

:::

-  $S_{AA}(\omega)$ can be interpreted in terms of Fermi golden rule, as we saw for oscillator. Notice that $S_{AA}(\omega)>0$

---

## Response of Matter

- Back to many body physics!

---

### Density Response

- Apply time dependent potential corresponding to term in Hamiltonian

$$
H_\text{pert} = \sum_{j=1}^N V(\br_i,t) = \int  V(\br,t)\rho(\br)\, d\br = \frac{1}{L^3}\sum_\bq V_\bq(t) \rho_{-\bq}
$$

- Perturbation couples to the density: how is density affected? 

- In a translationally invariant system

$$
\langle\langle \rho_\bq(t)\rangle\rangle = -\frac{1}{L^3} \int_{-\infty}^t  \chi^{\rho}_\bq(t-t') V_\bq(t)\,dt',
$$

where the density response function $\chi^\rho_\bq(t)$ is

$$
\chi_\rho(\bq,t) = i\langle\langle\left[\rho_\bq(t),\rho_{-\bq}(0)\right]\rangle\rangle
$$

---

- General theory applies with $A=\rho_\bq$ and $B=\rho_{-\bq}$. At $T=0$
$$
S_\rho(\bq,\omega) = 2\pi\sum_{n}  |\bra{0}\rho_\bq\ket{n}|^2 \delta(\omega-E_n+E_0)
$$

- This is the __dynamical structure factor__, on account of its importance in scattering experiments.

- The __static structure factor__ is
$$
S_\rho(\bq) = \int S_\rho(\bq,\omega) \frac{d\omega}{2\pi} = \langle\langle\rho_\bq\rho_{-\bq}\rangle\rangle
$$

---


### Sum rules

- $S_\rho(\bq,\omega)$ obeys certain general relations irrespective of system

- If interaction depends only on density $\left[H_\text{int},\rho_\bq\right]=0$

- $\left[H,\rho_\bq\right]=\left[T,\rho_\bq\right]$

$$
T = -\frac{1}{2m}\sum_{j=1}^N \nabla_i^2
$$

- Taking $\rho_\bq =\sum_{j=1}^N e^{-i\bq\cdot\br_j}$, we find

$$
[[H,\rho_\bq],\rho_{-\bq}] = -\frac{N\bq^2}{m}
$$

---

- Evaluate by introducing resolution of the identity $\sum_n \ket{n}\bra{n}=1$

$$
\begin{align*}
\braket{0|[[H,\rho_\bq],\rho_{-\bq}]|0}&=\braket{0|H\rho_\bq \rho_{-\bq}- \rho_\bq H\rho_{-\bq}-\rho_{-\bq} H\rho_\bq+\rho_{-\bq}\rho_\bq H|0}\\
&=2\sum_n|\bra{0}\rho_\bq\ket{n}|^2\left(E_0-E_n\right)
\end{align*}
$$

- We can relate this to $S(\bq,\omega)$ using spectral representation

$$
S_\rho(\bq,\omega) = 2\pi\sum_{n}  |\bra{0}\rho_\bq\ket{n}|^2 \delta(\omega-E_n+E_0)
$$
to give the __f-sum rule__

$$
\int_{-\infty}^\infty \omega S(\bq,\omega) \frac{d\omega}{2\pi}= \frac{N\bq^2}{2m}
$$


---

### Compressibility sum rule

- Compressibility

$$
\beta=-\frac{1}{V}\frac{\partial V}{\partial p}.
$$
(inverse of Bulk modulus)

- $p = -\frac{\partial E_0}{\partial V}$ at $T=0$. If $E_0 = V \epsilon(\rho)$, then

$$
\beta^{-1} = \rho^2 \epsilon''(\rho).
$$

---

$$
\beta^{-1} = \rho^2 \epsilon''(\rho).
$$

- In the presence of a potential $V(\br)$, energy density is 

$$
\epsilon(\rho_0+\delta\rho) = \frac{1}{2\beta\rho_0^2} \left[\delta\rho\right]^2 + V(\br)\delta\rho
$$

- Minimizing with respect to $\delta\rho$ gives

$$
\epsilon(V(\br)) = - \frac{\beta\rho_0^2}{2} \left[V(\br)\right]^2
$$

- Compare with perturbation theory

---

- Change in energy due to perturbation 

$$
\sum_j V_0 \cos(\bq\cdot \br_j) = \frac{V_0}{2}\left[\rho_\bq+\rho_{-\bq}\right] 
$$

- Second order perturbation theory for ground state
$$
E^{(2)} =\frac{V_0^2}{4} \sum_{n\neq 0} \frac{|\braket{0|\rho_\bq|n}|^2}{E_0-E_n} =-\frac{V_0^2}{4}\int_0^\infty \frac{S(\bq,\omega)}{\omega}\frac{d\omega}{2\pi}
$$
(first order vanishes)

---

- Compare with 

$$
\epsilon(V(\br)) = - \frac{\beta\rho_0^2}{2} \left[V(\br)\right]^2
$$

- This gives the __compressibility sum rule__ at zero temperature

$$
\lim_{\bq\to 0}\int_0^\infty \frac{S(\bq,\omega)}{\omega}\frac{d\omega}{2\pi} = \frac{N\rho\beta}{2}.
$$

- Compressibility sum rule often written in terms of speed of sound $c = (\beta m \rho)^{-1/2}$

$$
\lim_{\bq\to 0}\int_0^\infty \frac{S(\bq,\omega)}{\omega}\frac{d\omega}{2\pi} = \frac{N}{2mc^2}.
$$

---


### Single Mode Approximation

- Some systems (e.g Bose gases), are well described by
$$
S_\rho(\bq,\omega) \sim 2\pi S_\rho(\bq) \delta(\omega - \omega(\bq)),
$$
for low $\bq$, where $\omega(\bq)$ is dispersion relation of collective excitations (e.g. Bogoliubov modes)

- In this approximation, f-sum rule tells us that

$$
S_\rho(\bq) = \frac{N\bq^2}{2m\omega(\bq)}.
$$

---

### Example 1: BEC (no interactions)

- Excitations out of the condensate are free particles $\omega(\bq) = \frac{\bq^2}{2m}$
$$
S_\rho(\bq) = N.
$$

- Completely uncorrelated particle positions (Poisson statistics).

---

### Example 2: interacting BEC / elastic chain

- $\omega(\bq) = c|\bq|$ i.e. linear dispersion with finite speed of sound

$$
S_\rho(\bq) = \frac{N|\bq|}{2mc}.
$$

- Density fluctuations vanish as wavevector goes to zero, indicating long-range correlations between positions in the ground state.

::: {.callout-tip}
## Check

Check compressibility sum rule

:::

---

### Example 3: FQHE

- Assuming __single mode approximation__

$$
S_\rho(\bq,\omega) \sim 2\pi S_\rho(\bq) \delta(\omega - \omega(\bq))
$$

- Can use $S_\rho(\bq)$ to find dispersion (see e.g. @girvin2002quantum for FQHE)

$$
\omega(\bq) = \frac{N\bq^2}{2m S_\rho(\bq)}
$$

![](../assets/girvin-sma.png){width=40% fig-align="center"}